use Cancel.init_res & SMod.is_real

celliocb/CelliocbAll.v
@@ -1,93 +1,81 @@
-(* Require Import CRIS Cancel.
+Require Import CRIS Cancel.
 Require Import ImpPrelude.
 Require Import MaincbHeader.
 Require Import 
   CelliocbHeader CelliocbA CelliocbI MaincbA MaincbI CtxcbHeader CelliocbIAproof MaincbIAproof.
 
-Module CelliocbAll. Section CelliocbAll.
-  Import inv_instances.
-  Local Instance Γ : HRA := ##[invΓ; celliocbΓ].
-  Local Instance Σ : GRA := ##[Γ; invΣ].
-  Local Definition irΓ : Γ := **[ir_invΓ; CelliocbA.irΓ].
-  Local Definition irΣ : Σ := **[irΓ; ir_invΣ].
-  Lemma irΣ_valid : ✓ (irΣ ⋅ ir_own_admin).
-  Proof.
-    solve_ir_valid.
-    apply CelliocbA.ir_valid.
-  Qed.
+Section CelliocbAux.
+  Context `{!crisG Γ Σ α β τ Hsub Hinv, _CELL: !celliocbGS}.
 
-  Variable CtxcbI: SMod.t.
-  Hypothesis ctx_real: real_smod CtxcbI.
-  Hypothesis ctx_mod_wf: Mod.wf (SMod.to_mod sp_none CtxcbI).
-  Hypothesis ctx_smod_wf: SMod.wf CtxcbI.
-  Hypothesis ctx_has_foo: In (Some CtxcbHdr.foo) (map fst (SMod.fnsems CtxcbI)).
+  Variable CtxcbI : SMod.t.
+  Hypothesis ctx_real: SMod.is_real CtxcbI.
+  Hypothesis ctx_mod_wf: Mod.wf (SMod.to_mod ∅ CtxcbI).
+  Hypothesis ctx_cancellable : SMod.cancellable CtxcbI.
+  Hypothesis ctx_has_foo: fid CtxcbHdr.foo ∈ dom (SMod.fnsems CtxcbI).
   Hypothesis ctx_main_disj:
-    ∀ fno, In fno (map fst (SMod.fnsems CtxcbI)) → In fno (map fst (Mod.fnsems MaincbI.t)) → False.
+    ∀ fno, fno ∈ dom (SMod.fnsems CtxcbI) → fno ∈ dom (Mod.fnsems MaincbI.t) → False.
   Hypothesis ctx_cellio_disj:
-    ∀ fno, In fno (map fst (SMod.fnsems CtxcbI)) → In fno (map fst (Mod.fnsems CelliocbI.t)) → False.
+    ∀ fno, fno ∈ dom (SMod.fnsems CtxcbI) → fno ∈ dom (Mod.fnsems CelliocbI.t) → False.
   Hypothesis ctx_main_scope_disj:
-    ∀ mn, In mn (SMod.scopes CtxcbI) → In mn (Mod.scopes MaincbI.t) → False.
+    ∀ mn, mn ∈ (SMod.scopes CtxcbI) → mn ∈ (Mod.scopes MaincbI.t) → False.
   Hypothesis ctx_cellio_scope_disj:
-    ∀ mn, In mn (SMod.scopes CtxcbI) → In mn (Mod.scopes CelliocbI.t) → False.
-  
+    ∀ mn, mn ∈ (SMod.scopes CtxcbI) → mn ∈ (Mod.scopes CelliocbI.t) → False.
+
   Local Definition smod_src : SMod.t := MaincbA.smod ☆ CtxcbI.
-  Local Definition mod_top : Mod.t := SMod.to_mod sp_none (SMod.cancel smod_src).
-  Local Definition mod_tgt : Mod.t := MaincbI.t ★ CelliocbI.t ★ (SMod.to_mod sp_none CtxcbI).
+  Local Definition mod_top : Mod.t := SMod.to_mod ∅ (SMod.cancel smod_src).
 
-  Local Definition sp : sp_type := sp_from smod_src.
+  Local Definition sp : specmap := SMod.conc_sp_from smod_src.
   Local Definition mod_src : Mod.t := SMod.to_mod sp smod_src.
-  
+  Local Definition mod_tgt : Mod.t := MaincbI.t ★ CelliocbI.t ★ (SMod.to_mod sp CtxcbI).
+
   Local Definition init_cond : iProp Σ :=
-    winv (⊤, ⊤) ∗ MaincbA.init_cond ∗ CelliocbA.init_cond.
+    (CelliocbA.init_cond)%I.
 
-  Lemma sp_foo: sp CtxcbHdr.foo = None.
+  Lemma sp_foo: sp.1 !! fid CtxcbHdr.foo = None.
   Proof.
-    rewrite /sp /sp_from /to_sp /smod_src. s.
-    rewrite !alist_find_map_snd.
-    destruct (alist_find _ _) as [[[[? ?] ?] [? ?]]| ] eqn: E; ss.
-    - exploit (ctx_real (Some CtxcbHdr.foo)); et.
-    - assert (HAS:= ctx_has_foo). eapply in_map_iff in HAS.
-      des. destruct x. ss. subst.
-      exfalso. eapply alist_find_none in E; et.
+    rewrite /sp /SMod.conc_sp_from /= /smod_src /SMod.sp_core_from.
+    rewrite lookup_omap !lookup_fmap lookup_omap lookup_union_with.
+    assert (FIND: exists x, SMod.fnsems CtxcbI !! fid CtxcbHdr.foo = Some (Some x)).
+    { eapply elem_of_dom in ctx_has_foo. inv ctx_has_foo. eauto.
+      inv ctx_mod_wf. destruct x; eauto.
+      destruct (SMod.fnsems CtxcbI !! fid CtxcbHdr.foo) eqn:FIND; ss.
+      inv H. hexploit (wf_fns (fid CtxcbHdr.foo)).
+      { rewrite /Mod.fnsems /SMod.to_mod lookup_fmap FIND //. }
+      i. ss. inv H.
+    }
+    des. rewrite FIND. ss. destruct x, p. r in ctx_real. hexploit ctx_real; eauto.
   (*SLOW*)Qed.
-
+  
   (* Apply cancellation to linked spec module *)
   Lemma cancel_src:
-    refines (mod_top, init_cond) 
+    refines (mod_top, init_cond ∗ CelliocbA.cell 0 ∗ Cancel.init_res)%I
             (mod_src, init_cond).
-  Proof using ctx_main_disj ctx_main_scope_disj ctx_mod_wf ctx_real ctx_smod_wf.
+  Proof.
     eapply Cancel.cancellation; et.
-    - rewrite /smod_src. ii. destruct fno; ss.
-      + eapply ctx_smod_wf; et.
-      + inv FIND. et.
-    - split; try refl.
-      i. r in NS. des. r in NS. des.
-      rewrite /sp /smod_src /sp_from /to_sp. s.
-      rewrite !alist_find_map_snd.
-      destruct (alist_find (Some fn) _) eqn: E; s.
-      + destruct p as [[[img0 msk0] scp0] [fsp0 bd0]].
-        exploit ctx_real; et. i. subst.
-        eapply ctx_smod_wf in E. rewrite E; et.
-        s. refl.
-      + eapply fspec_bot_strongest.
-    - destruct ctx_mod_wf. econs; ss.
-      + econs.
-        * repeat (rewrite map_map; setoid_rewrite fst_map_snd).
-          ii. eapply ctx_main_disj; et.
-          unfold_mod. s. et.
-        * revert wf_fns.
-          repeat (rewrite map_map; setoid_rewrite fst_map_snd). et.
-      + econs; et.
-        ii. eapply ctx_main_scope_disj; et.
-        unfold_mod. s; et.
-  Qed.
+    { apply SMod.cancellable_add; r; rewrite /= /MaincbA.fnsems //; mod_tac ss. }
+    { assert (Ce : SMod.fnsems CtxcbI !! entry = None).
+      { eapply not_elem_of_dom. ii. eapply ctx_main_disj; eauto.
+        rewrite /MaincbI.t /MaincbI.smod /SMod.to_mod /= /Mod.fnsems. set_solver.
+      }
+      assert (Ht : (SMod.conc_sp_from smod_src).1 !! entry =
+        fsp_some MaincbA.main_spec); last (rewrite Ht; clear Ht).
+      { rewrite /SMod.conc_sp_from /SMod.sp_core_from.
+        rewrite !lookup_omap !lookup_fmap lookup_omap lookup_union_with.
+        simpl_map; ss. rewrite Ce //.
+      }
+      eexists _, _; splits.
+      { ss; exists tt; split; refl. }
+      { iIntros "($ & _ & [_ _])"; eauto. }
+      { unfold_pre_post. iIntros (??) "[$ _]". }
+    }
+  (*SLOW*)Qed.
 
   (* Refinement between spec/impl of whole program (linked module) *)
-  Lemma src_tgt : refines (mod_src, init_cond) (mod_tgt, emp%I).
-  Proof using ctx_has_foo ctx_mod_wf ctx_real ctx_smod_wf.
+  Lemma src_tgt : refines (mod_src, init_cond)%I (mod_tgt, emp%I).
+  Proof.
     eapply ctxr_refines.
     rewrite /init_cond /mod_src /smod_src /mod_tgt.
-    rewrite !add_interp_comm.
+    rewrite !SMod.to_mod_add.
     
     (* solve by transitivity:
       MaincbI ★ CelliocbI ⊆ MaincbI ★ CelliocbA ⊆ MaincbA ★ CelliocbA 
@@ -99,24 +87,22 @@ Module CelliocbAll. Section CelliocbAll.
     }
 
     etrans; cycle 1.
-    { (* MaincbI ★ CelliocbA ⊆ctx MaincbA *)
+    { (* MaincbI ★ CelliocbA ⊆ MaincbA *)
       ctxr_rotate. ctxr_drop. ctxr_rotate.
       eapply main_adequacy, MaincbIA.sim; eauto using sp_foo.
     }
 
     etrans; cycle 1.
-    { (* CtxI ⊆ CtxA *)
-      ctxr_rotate. ctxr_drop.
-      erewrite <-(@real_smod_ignores_sp _ CtxcbI sp); et. refl.
+    { (* CtxcbI ⊆ CtxcbI *)
+      ctxr_rotate. ctxr_drop. refl.
     }
-    
-    rewrite /MaincbIAproof.MaincbIA.MaincbA /MaincbA.t. unseal CRIS.
+
     eapply ctxr_cond_strengthen.
-    iIntros "[? ?]". iFrame.
+    iIntros "$".
   (*SLOW*)Qed.
 
   Lemma top_tgt :
-    refines (mod_top, init_cond)
+    refines (mod_top, init_cond ∗ CelliocbA.cell 0 ∗ Cancel.init_res)%I
             (mod_tgt, emp%I).
   Proof.
     etrans.
@@ -126,43 +112,85 @@ Module CelliocbAll. Section CelliocbAll.
 
   Lemma tgt_wf: Mod.wf mod_tgt.
   Proof.
-    revert_until CtxcbI. rewrite /mod_tgt /MaincbI.t /CelliocbI.t. unseal CRIS. i.
-    econs; s.
-    - prove_nodup.
-      + rewrite map_map in H. setoid_rewrite fst_map_snd in H. et.
-      + rewrite map_map in H. setoid_rewrite fst_map_snd in H. et.
-      + rewrite map_map in H. setoid_rewrite fst_map_snd in H. et.
-      + rewrite map_map in H. setoid_rewrite fst_map_snd in H. et.
-      + rewrite map_map in H. setoid_rewrite fst_map_snd in H. et.
-      + eapply ctx_mod_wf.
-    - prove_nodup.
-      + eapply ctx_cellio_scope_disj; et.
-      + eapply ctx_main_scope_disj; et.
-      + eapply ctx_mod_wf.
-  (*SLOW*)Qed.
-
-  Lemma init_cond_valid:
-    ∃ rs, ✓ rs ∧ (Own rs ⊢ init_cond).
-  Proof using.
-    exists (irΣ ⋅ ir_own_admin). split.
-    - apply irΣ_valid.
-    - simplify_res.
-      { rewrite make_own_admin; iFrame.
-        iDestruct "H12" as "[H2 H3]". iFrame.
+    rewrite /mod_tgt; eapply Mod.add_wf.
+    { econs; eauto; [mod_tac|prove_nodup]. }
+    { eapply Mod.add_wf.
+      { econs; eauto; [mod_tac|prove_nodup]. }
+      { inv ctx_mod_wf. econs.
+        { ii. destruct (SMod.fnsems CtxcbI !! i) eqn: FIND.
+          { rewrite /Mod.fnsems /SMod.to_mod lookup_fmap FIND /= in H. inv H.
+            destruct o; ss. hexploit (wf_fns i); eauto.
+            rewrite /Mod.fnsems /SMod.to_mod lookup_fmap FIND //.
+          }
+          { rewrite /Mod.fnsems /SMod.to_mod lookup_fmap FIND /= in H. inv H. }
+        }
+        { rewrite /SMod.to_mod /= in wf_scopes. rewrite /SMod.to_mod //. }
       }
-      all: solve_res.
-  Qed.
-    
-  Theorem behavioral_refinement :
-    ∃ src_res tgt_res, refines_lmod
-      (Mod.to_lmod mod_top src_res)
-      (Mod.to_lmod mod_tgt tgt_res).
-  Proof.
-    move: (top_tgt)=>H; rewrite /refines in H; des; ss.
-    hexploit H; eauto using tgt_wf. clear H; intros [WF H].
-    assert (IV:= init_cond_valid). des.
-    destruct (H rs); des; et.
-    rewrite IV0 /init_cond {1}winv_split_empty. iIntros "[[? ?] ?]". iFrame; done.
+      { ii. rewrite /Mod.fnsems /SMod.to_mod /= dom_fmap in H0. eauto. }
+      { eapply NoDup_app. esplits; eauto.
+        { prove_nodup. }
+        { inv ctx_mod_wf. rewrite /Mod.scopes /SMod.to_mod /= in wf_scopes.
+          rewrite /Mod.scopes /SMod.to_mod //.
+        }
+      }
+    }
+    { rewrite !Mod.dom_fnsems_add; set_solver. }
+    { eapply NoDup_app. esplits; eauto.
+      { prove_nodup. }
+      { ii. ss. rewrite sorting.merge_sort_Permutation in H0. set_solver. }
+      { ss. rewrite sorting.merge_sort_Permutation.
+        eapply NoDup_cons. esplits; eauto.
+        { ii. eapply ctx_cellio_disj; eauto. set_solver. }
+        { inv ctx_mod_wf. rewrite /Mod.scopes /SMod.to_mod /= in wf_scopes.
+          rewrite /Mod.scopes /SMod.to_mod //.
+        }
+      }
+    }
   (*SLOW*)Qed.
-End CelliocbAll. End CelliocbAll.
-Print Assumptions CelliocbAll.behavioral_refinement. *)
+End CelliocbAux.
+
+Module CelliocbAll.
+  Import inv_instances.
+
+  Local Instance Γ : HRA := ##[invΓ; concΓ; celliocbΓ].
+  Local Instance Σ : GRA := ##[Γ; invΣ].
+
+  Lemma behavioral_refinement :
+    ∃ β τ (Hinv : invGS Γ Σ α) (_ : crisG Γ Σ α β τ _ Hinv) (_ : celliocbGS),
+    ∀ (CtxcbI : SMod.t)
+      (ctx_real: SMod.is_real CtxcbI)
+      (ctx_mod_wf: Mod.wf (SMod.to_mod ∅ CtxcbI))
+      (ctx_cancellable : SMod.cancellable CtxcbI)
+      (ctx_has_foo: fid CtxcbHdr.foo ∈ dom (SMod.fnsems CtxcbI))
+      (ctx_main_disj:
+        ∀ fno, fno ∈ dom (SMod.fnsems CtxcbI) → fno ∈ dom (Mod.fnsems MaincbI.t) → False)
+      (ctx_cellio_disj:
+        ∀ fno, fno ∈ dom (SMod.fnsems CtxcbI) → fno ∈ dom (Mod.fnsems CelliocbI.t) → False)
+      (ctx_main_scope_disj:
+        ∀ mn, mn ∈ (SMod.scopes CtxcbI) → mn ∈ (Mod.scopes MaincbI.t) → False)
+      (ctx_cellio_scope_disj:
+        ∀ mn, mn ∈ (SMod.scopes CtxcbI) → mn ∈ (Mod.scopes CelliocbI.t) → False),
+    ∃ src_res tgt_res,
+    refines_lmod
+      (Mod.to_lmod (mod_top CtxcbI) src_res)
+      (Mod.to_lmod (mod_tgt CtxcbI) tgt_res).
+  Proof.
+    apply own_admin_soundness.
+    iMod cris_alloc as "[% [% [% [% ?]]]]".
+    iMod cellio_alloc as "[% ?]".
+    iExists _, _, _, _, _.
+    pose proof top_tgt as Href.
+    iStopProof. eapply entails_pointwise; iIntros (res Hres) "R".
+    iPoseProof (Own_valid with "R") as "%".
+    iPureIntro. i.
+    rewrite /refines in Href; hexploit Href; eauto using tgt_wf.
+    clear Href; intros [? Href].
+    hexploit (Href res); eauto.
+    { rewrite Hres. iIntros "((W & $ & $ & $ & $) & $ & $)".
+      rewrite {1}winv_split_empty comm //.
+    }
+    s; i; des; et.
+  (*SLOW*)Qed.
+End CelliocbAll.
+
+(* Print Assumptions CelliocbAll.behavioral_refinement. *)
